lib/Lang/LinearSequence.s.dfy
@@ -59,53 +59,53 @@ module {:extern "LinearExtern"} LinearSequence_s {
 
   type {:extern "predefined"} lseq<A>
 
-  function {:axiom} lseqs_raw<A>(l:lseq<A>):(s:seq<maybe<A>>) // contents of an lseq, as ghost seq
+  function {:axiom} lseqs_raw<A(00)>(l:lseq<A>):(s:seq<maybe<A>>) // contents of an lseq, as ghost seq
     ensures rank_is_less_than(s, l)
 
 
-  function lseq_has<A>(l:lseq<A>):(s:seq<bool>)
+  function lseq_has<A(00)>(l:lseq<A>):(s:seq<bool>)
       ensures |s| == |lseqs_raw(l)|
   {
     seq(|lseqs_raw(l)|, i requires 0 <= i < |lseqs_raw(l)| => has(lseqs_raw(l)[i]))
   }
 
 
-  lemma {:axiom} axiom_lseqs_rank<A>(l:lseq<A>, s:seq<A>)
+  lemma {:axiom} axiom_lseqs_rank<A(00)>(l:lseq<A>, s:seq<A>)
     requires |lseqs_raw(l)| == |s|
     requires forall i :: 0 <= i < |s| ==> s[i] == read(lseqs_raw(l)[i])
     ensures rank_is_less_than(s, l)
 
-  lemma {:axiom} axiom_lseqs_extensional<A>(l1:lseq<A>, l2:lseq<A>)
+  lemma {:axiom} axiom_lseqs_extensional<A(00)>(l1:lseq<A>, l2:lseq<A>)
     requires lseqs_raw(l1) == lseqs_raw(l2)
     ensures l1 == l2
 
   // it's okay to synthesize all the lseqs you want if they're ghosty
-  function {:axiom} imagine_lseq_raw<A>(s:seq<maybe<A>>):(l:lseq<A>)
+  function {:axiom} imagine_lseq_raw<A(00)>(s:seq<maybe<A>>):(l:lseq<A>)
     ensures lseqs_raw(l) == s
 
-  function method {:extern "LinearExtern", "lseq_length_raw"} lseq_length_raw<A>(shared s:lseq<A>):(n:uint64)
+  function method {:extern "LinearExtern", "lseq_length_raw"} lseq_length_raw<A(00)>(shared s:lseq<A>):(n:uint64)
     requires |lseqs_raw(s)| <= 0xffff_ffff_ffff_ffff
     ensures n as int == |lseqs_raw(s)|
 
-  function method {:extern "LinearExtern", "lseq_alloc_raw"} lseq_alloc_raw<A>(length:uint64):(linear s:lseq<A>)
+  function method {:extern "LinearExtern", "lseq_alloc_raw"} lseq_alloc_raw<A(00)>(length:uint64):(linear s:lseq<A>)
       ensures |lseqs_raw(s)| == length as nat
       ensures forall i:nat | i < length as nat :: !has(lseqs_raw(s)[i])
 
-  function method {:extern "LinearExtern", "lseq_free_raw"} lseq_free_raw<A>(linear s:lseq<A>):()
+  function method {:extern "LinearExtern", "lseq_free_raw"} lseq_free_raw<A(00)>(linear s:lseq<A>):()
       requires forall i:nat | i < |lseqs_raw(s)| :: !has(lseqs_raw(s)[i])
 
   // can be implemented as in-place swap
-  function method {:extern "LinearExtern", "lseq_swap_raw_fun"} lseq_swap_raw_fun<A>(linear s1:lseq<A>, i:uint64, linear a1:maybe<A>):(linear p:(linear lseq<A>, linear maybe<A>))
+  function method {:extern "LinearExtern", "lseq_swap_raw_fun"} lseq_swap_raw_fun<A(00)>(linear s1:lseq<A>, i:uint64, linear a1:maybe<A>):(linear p:(linear lseq<A>, linear maybe<A>))
       requires i as int < |lseqs_raw(s1)|
       ensures p.1 == lseqs_raw(s1)[i]
       ensures lseqs_raw(p.0) == lseqs_raw(s1)[i as int := a1]
 
-  function method {:extern "LinearExtern", "lseq_share_raw"} lseq_share_raw<A>(shared s:lseq<A>, i:uint64):(shared a:maybe<A>)
+  function method {:extern "LinearExtern", "lseq_share_raw"} lseq_share_raw<A(00)>(shared s:lseq<A>, i:uint64):(shared a:maybe<A>)
       requires i as int < |lseqs_raw(s)|
       ensures a == lseqs_raw(s)[i]
 
   // must be a method, not a function method, so that we know s is a run-time value, not a ghost value
-  method {:extern "LinearExtern", "lseq_length_bound"} lseq_length_bound<A>(shared s:lseq<A>)
+  method {:extern "LinearExtern", "lseq_length_bound"} lseq_length_bound<A(00)>(shared s:lseq<A>)
     ensures |lseqs_raw(s)| < 0xffff_ffff_ffff_ffff
 
   method {:extern "LinearExtern", "TrustedRuntimeSeqResize"} TrustedRuntimeSeqResize<A>(linear s: seq<A>, newlen: uint64)
@@ -113,7 +113,7 @@ module {:extern "LinearExtern"} LinearSequence_s {
     ensures |s2| == newlen as nat
     ensures forall j :: 0 <= j < newlen as nat && j < |s| ==> s2[j] == s[j]
 
-  method {:extern "LinearExtern", "TrustedRuntimeLSeqResize"} TrustedRuntimeLSeqResize<A>(linear s: lseq<A>, newlen: uint64)
+  method {:extern "LinearExtern", "TrustedRuntimeLSeqResize"} TrustedRuntimeLSeqResize<A(00)>(linear s: lseq<A>, newlen: uint64)
     returns (linear s2: lseq<A>)
     ensures |lseqs_raw(s2)| == newlen as nat
     ensures forall j :: 0 <= j < newlen as nat && j < |lseqs_raw(s)| ==> lseq_has(s2)[j] == lseq_has(s)[j]
